Sketch some proofs on simplified definitions
Instead of working with the "old" definitions, we give alternative
definitions, essentially identical, with very minor differences, that
make use of the revised definitions. The properties to be proved are
almost identical, but some of the constituent results --illustrated here
by the domain preservation lemmas-- now follow directly from the new
formulation.

Intermediate/Machine.v
@@ -633,6 +633,42 @@ Definition prepare_procedures_memory (p: program) (mem: Memory.t) : Memory.t :=
 
 (* Lemma placeholder: prepare_procedures_memory_after_linking *)
 
+Definition prepare_procedures_memory' (p: program) : Memory.t :=
+  let '(mem, _, _) := prepare_procedures_initial_memory p in
+  mem.
+
+(* First, prove domain preservation for all of the (already existing, plus
+   recent improvements) initialization code. *)
+Lemma domm_prepare_procedures_initial_memory_aux: forall p,
+  (*well_formed_program p ->*)
+  domm (prepare_procedures_initial_memory_aux p) = domm (prog_interface p).
+Proof.
+  intros p.
+  unfold prepare_procedures_initial_memory_aux.
+  rewrite domm_mkfmapf.
+Admitted. (* Grade 1. *)
+
+(* Now it's easy to extend this to the parts of the final result. *)
+Lemma domm_prepare_procedures_memory': forall p,
+  domm (prepare_procedures_memory' p) = domm (prog_interface p).
+Proof.
+  intros p.
+  unfold prepare_procedures_memory', prepare_procedures_initial_memory.
+  rewrite domm_map.
+  rewrite domm_prepare_procedures_initial_memory_aux.
+  reflexivity.
+Qed.
+
+(* RB: TODO: Simplify hypotheses if possible. *)
+Theorem prepare_procedures_memory_after_linking':
+  forall p c,
+    well_formed_program p ->
+    well_formed_program c ->
+    linkable (prog_interface p) (prog_interface c) ->
+    prepare_procedures_memory' (program_link p c) =
+    unionm (prepare_procedures_memory' p) (prepare_procedures_memory' c).
+Admitted.
+
 Definition prepare_procedures_entrypoints (p: program) (mem: Memory.t) : EntryPoint.t :=
   let '(_, _, entrypoints) := prepare_procedures p mem in
   entrypoints.
